src/Imp.v
@@ -1,13 +1,12 @@
 (*! Definition of a small imperative language !*)
 
-From PresburgerAI Require Export TotalMap EqDec RelationalAbstractDomain.
+From PresburgerAI Require Export TotalMap EqDec RelationalAbstractDomain Utils.
 From Coq Require Export Strings.String ZArith List.
 
 Open Scope list_scope.
-Open Scope Z_scope.
 
 (** Variables id **)
-Definition Vid := string.
+Notation Vid n := (Fin n).
 
 (** Location ids **)
 Definition Location := list nat.
@@ -16,25 +15,27 @@ Definition Location := list nat.
 Inductive BinOpCode := Add | Mul | Le.
 
 (** A Program **)
-Inductive Program :=
-| PBinop (res: Vid) (opc: BinOpCode) (op1 op2: Vid)
+Inductive Program {n: nat} :=
+| PBinop (res: Vid n) (opc: BinOpCode) (op1 op2: Vid n)
 | PSeq (p1 p2: Program)
-| PIf (cond_var: Vid) (p_true p_false: Program)
-| PWhile (cond: Vid) (p1: Program).
+| PIf (cond_var: Vid n) (p_true p_false: Program)
+| PWhile (cond: Vid n) (p1: Program).
+
+Arguments Program : clear implicits.
 
 (** A state in the program **)
-Notation State := (TotalMap Vid Z).
+Notation State n := (TotalMap (Vid n) Z).
 
 (** Execute a binary operation given both operands values **)
 Definition execute_binop (opc: BinOpCode) (v1 v2: Z) :=
   match opc with
-  | Add => v1 + v2
-  | Mul => v1 * v2
-  | Le => if v1 <=? v2 then 1 else 0
+  | Add => (v1 + v2)%Z
+  | Mul => (v1 * v2)%Z
+  | Le => if (v1 <=? v2)%Z then 1%Z else 0%Z
   end.
 
 (** Execute a binary operation on a state **)
-Definition execute_binop_state (opc: BinOpCode) (op1 op2: Vid) (s: State) :=
+Definition execute_binop_state {n: nat} (opc: BinOpCode) (op1 op2: Vid n) (s: State n) :=
   execute_binop opc (s op1) (s op2).
 
 (** Notation for relational semantics **)
@@ -43,37 +44,37 @@ Reserved Notation
          (at level 40, st constr, st' constr at next level).
 
 (** Relational semantics of a program **)
-Inductive semantics : Program -> State -> State -> Prop :=
+Inductive semantics {n: nat} : Program n -> State n -> State n -> Prop :=
 | EBinop res opc op1 op2 s :
   s =[ PBinop res opc op1 op2 ]=> (res !!-> execute_binop_state opc op1 op2 s; s)
 | ESeq p1 p2 s s' s'' :
     s =[ p1 ]=> s' ->
     s' =[ p2 ]=> s'' ->
     s =[ PSeq p1 p2 ]=> s''
-| EIfTrue var p_true p_false (s s': State) :
-    (s var) <> 0 ->
+| EIfTrue var p_true p_false (s s': State n) :
+    (s var) <> 0%Z ->
     s =[ p_true ]=> s' ->
     s =[ PIf var p_true p_false ]=> s'
-| EIfFalse var p_true p_false (s s': State) :
-    (s var) = 0 ->
+| EIfFalse var p_true p_false (s s': State n) :
+    (s var) = 0%Z ->
     s =[ p_false ]=> s' ->
     s =[ PIf var p_true p_false ]=> s'
-| EWhileTrue var p (s s' s'': State) :
-    (s var) <> 0 ->
+| EWhileTrue var p (s s' s'': State n) :
+    (s var) <> 0%Z ->
     s =[ p ]=> s' ->
     s' =[ PWhile var p ]=> s'' ->
     s =[ PWhile var p ]=> s''
-| EWhileFalse var p (s: State) :
-    (s var) = 0 ->
+| EWhileFalse var p (s: State n) :
+    (s var) = 0%Z ->
     s =[ PWhile var p ]=> s
 where "st =[ p ]=> st'" := (semantics p st st').
 
 Section ImpLemmas.
 
   (** When we are out of the while loop, the condition is false **)
-  Lemma while_out_cond cond p s s' :
-    s =[ PWhile cond p ]=> s' ->
-    s' cond = 0.
+  Lemma while_out_cond n cond p s s' :
+    s =[ @PWhile n cond p ]=> s' ->
+    s' cond = 0%Z.
   Proof.
     intros.
     remember (PWhile _ _).
@@ -81,9 +82,9 @@ Section ImpLemmas.
   Qed.
 
   (** equivalence with the denotational semantics**)
-  Lemma while_trans_closure cond p s s' :
-    s =[ PWhile cond p ]=> s' <->
-    transitive_closure (fun (s: State * State) => ((fst s) cond <> 0) /\ (fst s) =[ p ]=> (snd s)) (s, s') /\ s' cond = 0.
+  Lemma while_trans_closure n cond p s s' :
+    s =[ @PWhile n cond p ]=> s' <->
+    transitive_closure (fun (s: State n * State n) => ((fst s) cond <> 0%Z) /\ (fst s) =[ p ]=> (snd s)) (s, s') /\ s' cond = 0%Z.
   Proof.
     split; intros.
     - split; [ | eauto using while_out_cond ].
