src/TransferFunction.v
@@ -3,31 +3,32 @@ From PresburgerAI Require Export RelationalAbstractDomain Imp.
 Section TransferFunctionDefinition.
 
   Context {AbstractState: Type}
-          {adom: AbstractDomain (State * State) AbstractState}.
+          {n: nat}
+          {adom: AbstractDomain (State n * State n) AbstractState}.
 
   (** Properties on abstract domain to be able to use the abstract interpreter
       for Imp **)
   Class TransferFunction :=
   {
-    transfer_binop : Vid -> BinOpCode -> Vid -> Vid -> AbstractState;
+    transfer_binop : Vid n -> BinOpCode -> Vid n -> Vid n -> AbstractState;
     transfer_binop_sound :
       forall res opc op1 op2 s s',
         s =[ PBinop res opc op1 op2 ]=> s' ->
         in_dom (s, s') (transfer_binop res opc op1 op2);
 
-    filter_true_value : Vid -> AbstractState;
+    filter_true_value : Vid n -> AbstractState;
     filter_true_value_sound :
-      forall (var: Vid) (s: State),
-        (s var) <> 0 ->
+      forall (var: Vid n) (s: State n),
+        (s var) <> 0%Z ->
         in_dom (s, s) (filter_true_value var);
 
-    filter_false_value : Vid -> AbstractState;
+    filter_false_value : Vid n -> AbstractState;
     filter_false_value_sound :
-      forall (var: Vid) (s: State),
-        (s var) = 0 ->
+      forall (var: Vid n) (s: State n),
+        (s var) = 0%Z ->
         in_dom (s, s) (filter_false_value var)
   }.
 
 End TransferFunctionDefinition.
 
-Arguments TransferFunction {AbstractState} adom.
+Arguments TransferFunction {AbstractState} {n} adom.
